cedar-lean/Cedar/Thm/Validation/Levels.lean
@@ -1,0 +1,194 @@
+import Cedar.Thm.Data.Map
+import Cedar.Thm.Validation.Typechecker.Basic
+import Cedar.Thm.Validation.Typechecker.And
+import Cedar.Thm.Validation.Typechecker.GetAttr
+import Cedar.Thm.Validation.Typechecker.HasAttr
+import Cedar.Thm.Validation.Typechecker.Record
+import Cedar.Thm.Validation.Typechecker.Set
+import Cedar.Thm.Validation.Typechecker.Call
+import Cedar.Thm.Validation.Typechecker
+import Cedar.Thm.Validation.Levels.Soundness
+import Cedar.Thm.Validation.Levels.Util
+
+
+namespace Cedar.Thm
+
+open Cedar.Data
+open Cedar.Spec
+open Cedar.Validation
+
+-- Main soundness theorem of the leveled type system
+-- If you type check with an non-finite level
+-- And you provide a well formed store
+-- Then the only erors you can get are arithmatic/extension errors
+theorem type_of_is_sound_noninfinite {e : Expr} {c₁ c₂ : Capabilities} {env : Environment} {ty : CedarType} {request : Request} {entities : Entities} {l : Level} :
+  l < .infinite →
+  CapabilitiesInvariant c₁ request entities →
+  RequestAndEntitiesMatchEnvironmentLeveled env request entities l →
+  typeOf e c₁ env (l == .infinite) = .ok (ty, c₂) →
+  GuardedCapabilitiesInvariant e c₂ request entities ∧
+  ∃ (v : Value), EvaluatesToLeveled e request entities v ∧ InstanceOfType v ty
+  := by
+  intros h_level_finite h_caps h_reqs_levels h_typeof
+  have h_reqs := request_and_entity_match_level_implies_regular h_reqs_levels
+
+  have h_sound := (@ type_of_is_sound e) h_caps h_reqs h_typeof
+  have ⟨h_sound₁, v, _, _⟩ := h_sound
+  clear h_sound
+  cases e
+  case lit =>
+    apply type_of_is_sound_noninfinite_lit
+    repeat assumption
+  case var x _ =>
+    apply type_of_is_sound_noninfinite_var x h_caps h_reqs_levels h_typeof
+  case ite =>
+    apply type_of_is_sound_noninfinite_ite
+    repeat assumption
+    case _ =>
+      prove_ih type_of_is_sound_noninfinite
+    case _ =>
+      prove_ih type_of_is_sound_noninfinite
+    case _ =>
+      prove_ih type_of_is_sound_noninfinite
+  case and =>
+    apply type_of_is_sound_noninfinite_and
+    repeat assumption
+    case _ =>
+      prove_ih type_of_is_sound_noninfinite
+    case _ =>
+      prove_ih type_of_is_sound_noninfinite
+  case or =>
+    apply type_of_is_sound_noninfinite_or
+    repeat assumption
+    case _ =>
+      prove_ih type_of_is_sound_noninfinite
+    case _ =>
+      prove_ih type_of_is_sound_noninfinite
+  case getAttr =>
+    apply type_of_is_sound_noninfinite_getAttr
+    repeat assumption
+    prove_ih type_of_is_sound_noninfinite
+  case unaryApp =>
+    apply type_of_is_sound_noninfinite_unary
+    repeat assumption
+    prove_ih type_of_is_sound_noninfinite
+  case binaryApp =>
+    apply type_of_is_sound_noninfinite_binary
+    repeat assumption
+    prove_ih type_of_is_sound_noninfinite
+    prove_ih type_of_is_sound_noninfinite
+  case hasAttr =>
+    apply type_of_is_sound_noninfinite_hasAttr
+    repeat assumption
+    prove_ih type_of_is_sound_noninfinite
+  case set =>
+    apply type_of_is_sound_noninfinite_set
+    repeat assumption
+    intros
+    prove_ih type_of_is_sound_noninfinite
+  case record =>
+    apply type_of_is_sound_noninfinite_record
+    repeat assumption
+    intros
+    prove_ih type_of_is_sound_noninfinite
+  case call =>
+    apply type_of_is_sound_noninfinite_call
+    repeat assumption
+    intros
+    prove_ih type_of_is_sound_noninfinite
+termination_by sizeOf e
+decreasing_by
+  all_goals simp_wf
+  all_goals (try omega)
+  case _ =>
+    rename e = (.ite _ _ _) => heq
+    simp [heq]
+    omega
+  case _ =>
+    rename e = (.ite _ _ _) => heq
+    simp [heq]
+    omega
+  case _ =>
+    rename e = (.ite _ _ _) => heq
+    simp [heq]
+    omega
+  case _ =>
+    rename e = (.and _ _) => heq
+    simp [heq]
+    omega
+  case _ =>
+    rename e = (.and _ _) => heq
+    simp [heq]
+    omega
+  case _ =>
+    rename e = (.or _ _) => heq
+    simp [heq]
+    omega
+  case _ =>
+    rename e = (.or _ _) => heq
+    simp [heq]
+    omega
+  case _ =>
+    rename e = .unaryApp _ _ => heq
+    simp [heq]
+    omega
+  case _ =>
+    rename e = .binaryApp _ _ _ => heq
+    simp [heq]
+    omega
+  case _ =>
+    rename e = .binaryApp _ _ _ => heq
+    simp [heq]
+    omega
+  case _ =>
+    rename e = .getAttr _ _ => heq
+    simp [heq]
+    omega
+  case _ =>
+    rename e = .hasAttr _ _ => heq
+    simp [heq]
+    omega
+  case _ =>
+    rename List Expr => members
+    rename _ = Expr.set _ => heq
+    rename _ ∈ members => hin
+    rename Expr => e'
+    have size₁ : sizeOf e' < sizeOf members := by
+      apply List.in_lists_means_smaller
+      assumption
+    have size₂ : sizeOf members < sizeOf (Expr.set members) := by
+      simp
+      omega
+    rw [← heq] at size₂
+    omega
+  case _ =>
+    rename List (Attr × Expr) => members
+    rename _ = Expr.record members => heq
+    rename Expr => e'
+    rename Attr => a
+    have step₁ : sizeOf e' < sizeOf (a,e') := by
+      simp
+      omega
+    have step₂ : sizeOf (a,e') < sizeOf members := by
+      apply List.in_lists_means_smaller
+      assumption
+    have step₃ : sizeOf members < sizeOf (Expr.record members) := by
+      simp
+      omega
+    rw [← heq] at step₃
+    omega
+  case _ =>
+    rename List Expr => args
+    rename _ = Expr.call _ args => heq
+    rename ExtFun => xfn
+    rename Expr => e'
+    have step₁ : sizeOf e' < sizeOf args := by
+      apply List.in_lists_means_smaller
+      assumption
+    have step₂ : sizeOf args < sizeOf (Expr.call xfn args) := by
+      simp
+      omega
+    rw [← heq] at step₂
+    omega
+
+end Cedar.Thm
