cedar-lean/Cedar/Thm/Validation/Levels/Util.lean
@@ -1,0 +1,298 @@
+import Cedar.Thm.Data.Map
+import Cedar.Thm.Validation.Typechecker.Basic
+import Cedar.Thm.Validation.Typechecker.And
+import Cedar.Thm.Validation.Typechecker.GetAttr
+import Cedar.Thm.Validation.Typechecker.HasAttr
+import Cedar.Thm.Validation.Typechecker.Record
+import Cedar.Thm.Validation.Typechecker.Set
+import Cedar.Thm.Validation.Typechecker.Call
+import Cedar.Thm.Validation.Typechecker
+
+namespace Cedar.Thm
+
+open Cedar.Data
+open Cedar.Spec
+open Cedar.Validation
+
+theorem level_non_infite {l : Level} :
+  l < .infinite →
+  (l == .infinite) = false := by
+  intros h
+  cases h
+  simp
+  unfold Not
+  intros
+  contradiction
+
+theorem entity_find {entities : Entities} {attrs : Map Attr Value} {uid : EntityUID}
+  (h : entities.attrs uid = Except.ok attrs) :
+  ∃ e, entities.find? uid = some e
+  := by
+  unfold Entities.attrs at h
+  unfold Map.findOrErr at h
+  cases hfind : (Map.find? entities uid) <;> rw [hfind] at h <;> simp at h
+  rename_i val
+  exists val
+
+theorem lt_trans {l₁ l₂ l₃ : Level}
+  (h₁ : l₁ < l₂)
+  (h₂ : l₂ < l₃) :
+  l₁ < l₃ := by
+  cases h₁ <;> cases h₂
+  case _ n₁ n₂ h₁ n₂' h₂ =>
+    apply LevelLT.finite₁
+    omega
+  case _ h₁ h₂ =>
+    apply LevelLT.finite₂
+
+theorem le_trans {l₁ l₂ l₃ : Level}
+  (h₁ : l₁ ≤ l₂)
+  (h₂ : l₂ ≤ l₃) :
+  l₁ ≤ l₃ := by
+  simp [LE.le] at h₁
+  simp [LE.le] at h₂
+  simp [LE.le]
+  cases h₁ <;> cases h₂
+  case _ h₁ h₂ =>
+    simp [h₁, h₂]
+  case _ h₁ h₂ =>
+    simp [h₁, h₂]
+  case _ h₁ h₂ =>
+    subst h₂
+    simp [h₁]
+  case _ h₁ h₂ =>
+    apply Or.inr
+    apply lt_trans
+    repeat assumption
+
+theorem le_infinite {l : Level} :
+  .infinite ≤ l →
+  l = .infinite := by
+  intros h
+  cases l <;> try rfl
+  cases h
+
+theorem zero_le_all : ∀ (l : Level),
+  .finite 0 ≤ l := by
+  intros l
+  simp [LE.le]
+  cases l
+  case _ =>
+    apply Or.inr
+    apply LevelLT.finite₂
+  case _ n =>
+    cases n
+    case _ =>
+      simp [Level.finite]
+    case _ =>
+      apply Or.inr
+      apply LevelLT.finite₁
+      omega
+
+theorem le_lift : ∀ (n₁ n₂ : Nat),
+  n₁ ≤ n₂ →
+  Level.finite n₁ ≤ .finite n₂ := by
+  intros n₁ n₂ h
+  cases heq : decide (n₁ = n₂)  <;> simp at heq
+  case _ =>
+    have lt : n₁ < n₂ := by omega
+    simp [LE.le]
+    apply Or.inr
+    apply LevelLT.finite₁
+    assumption
+  case _ =>
+    subst heq
+    simp [LE.le]
+
+theorem all_le_infinit : ∀ (l : Level),
+  l ≤ .infinite := by
+  intros l
+  simp [LE.le]
+  cases l
+  case _ =>
+    simp [Level.infinite]
+  case _ =>
+    apply Or.inr
+    apply LevelLT.finite₂
+
+theorem lub_not_record : ∀ rty₁ rty₂ ty,
+  (.record rty₁ ⊔ .record rty₂) = some ty →
+  (match ty with
+    | .record _ => false
+    | _ =>true
+  ) = true →
+  False
+  := by
+  intros rty₁ rty₂ ty h₁ h₂
+  unfold lub? at h₁
+  cases hlub : lubRecordType rty₁.1 rty₂.1
+  case _ =>
+    simp [hlub] at h₁
+  case _ =>
+    simp [hlub] at h₁
+    subst h₁
+    simp at h₂
+
+-- macro "solve_var" v:(ident) l₁:(ident) l₂:(ident) : tactic => do
+macro "not_record" : tactic => do
+  `(tactic | (
+    exfalso
+    apply lub_not_record
+    assumption
+    simp
+  ))
+
+theorem qualitype_lub_lifts  {qty₁ qty₂ qty : QualifiedType}
+  (h : lubQualifiedType qty₁ qty₂ = some qty) :
+  (qty₁.getType ⊔ qty₂.getType) = some qty.getType
+  := by
+  cases qty₁ <;> cases qty₂
+    <;> simp [lubQualifiedType, Option.bind] at h
+    <;> rename_i ty₁ ty₂
+    <;> cases hlub : (ty₁ ⊔ ty₂) <;> simp [hlub] at h
+    <;> subst h
+    <;> simp [Qualified.getType]
+    <;> assumption
+
+theorem bounded_above {l₁ l₂ : Level} :
+  l₁ < .infinite →
+  l₁ ≥ l₂ →
+  l₂ < .infinite
+  := by
+  intros h₁ h₂
+  cases l₁ <;> cases l₂ <;> try cases h₁
+  cases h₂
+  apply LevelLT.finite₂
+
+theorem lt_zero_gt_zero_false {l : Level}
+  (h₁ : l > .finite 0)
+  (h₂ : l ≤ .finite 0) :
+  False := by
+  cases l
+  case none => -- l = infinity
+    cases h₂
+  case some n =>
+    simp [LE.le] at h₂
+    cases h₂
+    case _ heq =>
+      simp [Level.finite] at heq
+      subst heq
+      cases h₁
+      omega
+    case _ hlt =>
+      cases h₁
+      cases hlt
+      omega
+
+theorem lt_zero_helper {l₁ l₂ : Level}
+  (h₁ : l₂ > .finite 0)
+  (h₂ : l₁ ≥ l₂) :
+  l₁ ≠ .finite 0
+  := by
+  simp at h₁
+  simp [LE.le] at h₂
+  cases h₂
+  case _ h₂ =>
+    subst h₂
+    simp
+    intros h
+    subst h
+    cases h₁
+    omega
+  case _ h₂ =>
+    cases l₁ <;> cases l₂
+    case _ =>
+      simp
+      contradiction
+    case _ n₁  =>
+      simp
+      intros h
+      contradiction
+    case _ n₂ =>
+      cases h₂
+    case _ n₁ n₂ =>
+      cases h₂
+      rename_i h₂
+      cases h₁
+      rename_i h₁
+      have hzero : n₁ ≠ 0 := by omega
+      simp
+      intros contra
+      apply hzero
+      simp [Level.finite] at contra
+      assumption
+
+theorem gt_zero_helper
+  (l : Level)
+  (h₁ : l > .finite 0) :
+  l ≠ .finite 0 := by
+  cases l
+  case _ =>
+    simp [Level.finite]
+  case _ n =>
+    cases h₁
+    simp [Level.finite]
+    omega
+
+theorem zero_contra {l : Level}
+  (h₁ : l > .finite 0)
+  (h₂ : l ≤ .finite 0) :
+  False
+  := by
+  simp [LE.le] at h₂
+  cases h₂
+  case _ h₂ =>
+    subst h₂
+    cases h₁
+    omega
+  case _ h₂ =>
+    simp at h₁
+    cases l
+    case _ =>
+      cases h₂
+    case _ n =>
+      cases h₂
+      omega
+
+-- We repeat this proof a lot
+macro "type_soundness" : tactic =>
+  `(tactic | (
+    apply type_of_is_sound
+    assumption
+    apply request_and_entity_match_level_implies_regular
+    assumption
+    repeat assumption
+  ))
+
+-- Repeat case analysis
+macro "dril_to_value" hsound₂:(ident) h₅:(ident) : tactic =>
+  `(tactic |  (
+      have hsound₂ := $hsound₂
+      have h₅ := $h₅
+      cases hsound₂ <;> rename_i hsound₂ <;> try simp [hsound₂] at h₅
+      cases hsound₂ <;> rename_i hsound₂ <;> try simp [hsound₂] at h₅
+      cases hsound₂ <;> rename_i hsound₂ <;> try simp [hsound₂] at h₅
+      clear hsound₂
+      subst h₅
+  ))
+
+-- Lisp style car,caar,cddr macros but for ∨
+
+macro "inrr" : tactic =>
+  `(tactic | (
+    apply Or.inr
+    apply Or.inr
+    ))
+
+macro "inrl" : tactic =>
+  `(tactic | (
+    apply Or.inr
+    apply Or.inl
+    ))
+
+macro "inl" : tactic =>
+  `(tactic | (
+    apply Or.inl
+    ))
+
+end Cedar.Thm
