cedar-lean/Cedar/Thm/Validation/Levels/WellFormed.lean
@@ -1,0 +1,1264 @@
+
+import Cedar.Thm.Validation.Typechecker.Basic
+import Cedar.Thm.Validation.Typechecker.And
+import Cedar.Thm.Validation.Typechecker.GetAttr
+import Cedar.Thm.Validation.Typechecker.HasAttr
+import Cedar.Thm.Validation.Typechecker.Record
+import Cedar.Thm.Validation.Typechecker.Set
+import Cedar.Thm.Validation.Typechecker.Call
+import Cedar.Thm.Data.Map
+import Cedar.Thm.Validation.Typechecker
+import Cedar.Thm.Validation.Levels.Util
+
+namespace Cedar.Thm
+
+open Cedar.Data
+open Cedar.Spec
+open Cedar.Validation
+
+-- This is the central property we will be proving here
+-- If you start from a well formed entity store and evaluate an expression
+-- Then you should end up with a value/type that is well formed
+def EvaluatesToWellFormed (x : Expr) : Prop :=
+  ∀ (v : Value) (ty : CedarType) (request : Request)
+  (env : Environment)
+  (entities : Entities) (c₁ c₂ : Capabilities)  (l₁ : Level),
+  l₁ < .infinite →
+  RequestAndEntitiesMatchEnvironmentLeveled env request entities l₁ →
+  typeOf x c₁ env (l₁ == .infinite) = Except.ok (ty, c₂) →
+  evaluate x request entities = Except.ok v →
+  CapabilitiesInvariant c₁ request entities →
+   (entities ⊢ v : ty)
+
+-- A well formed value/type is still well formed at its lub
+theorem levels_lub {entities : Entities} {v : Value} {ty₁ ty₂ ty : CedarType}
+  (h₁ : (ty₁ ⊔ ty₂) = some ty)
+  (h₂ : entities ⊢ v : ty₁)  :
+  (entities ⊢ v : ty) := by
+  cases ty₁ <;> cases ty₂ <;> cases ty
+    <;> try simp [lub?, lubBool, Option.bind] at h₁
+    <;> try simp [lub?, lubBool, Option.bind] at h₂
+  case _ =>
+    rename_i bty₁ bty₂ bty
+    cases bty₁ <;> cases bty₂ <;> cases bty
+      <;> try simp [lub?, lubBool] at h₁ <;> try assumption
+    case _ =>
+      cases h₂
+      rename_i b h₁
+      cases b <;> simp [InstanceOfBoolType] at h₁
+      apply WellFormed.bool
+      simp [InstanceOfBoolType]
+    case _ =>
+      cases h₂
+      rename_i b h₁
+      cases b <;> simp [InstanceOfBoolType] at h₁
+      apply WellFormed.bool
+      simp [InstanceOfBoolType]
+    case _ =>
+      cases h₂
+      rename_i b h₁
+      cases b <;> simp [InstanceOfBoolType] at h₁
+      apply WellFormed.bool
+      simp [InstanceOfBoolType]
+    case _ =>
+      cases h₂
+      rename_i b h₁
+      cases b <;> simp [InstanceOfBoolType] at h₁
+      apply WellFormed.bool
+      simp [InstanceOfBoolType]
+  case _ =>
+    assumption
+  case _ =>
+    assumption
+  case _ =>
+    rename_i ty₁ l₁ ty₂ l₂ ty l
+    replace ⟨h₁, h₃, h₄⟩ := h₁
+    subst h₁
+    subst h₃
+    subst h₄
+    cases h₂
+    case entity₀ euid h₁ =>
+      cases l₂ <;> simp [min, Option.min, Level.finite, none]
+        <;> apply WellFormed.entity₀
+        <;> assumption
+    case entityₙ euid attrs heq h₂ h₃ h₁ =>
+      apply WellFormed.entityₙ
+      assumption
+      assumption
+      intros k v t' hin
+      apply h₂
+      assumption
+      intros k v t' hin
+      have hstep : level t' ≥ l₁.sub1 := by apply h₁ ; repeat assumption
+      cases l₁ <;> cases l₂
+      case _ =>
+        simp [Level.sub1] at hstep
+        have hinf := le_infinite hstep
+        rw [hinf]
+        simp [LE.le, min, Option.min, Level.sub1, Level.infinite]
+      case _ =>
+        rename_i n
+        simp [min, Option.min]
+        have hinf := le_infinite hstep
+        rw [hinf]
+        apply all_le_infinit
+      case _ =>
+        rename_i n
+        simp [min, Option.min]
+        simp at hstep
+        assumption
+      case _ n₁ n₂ =>
+        cases n₁ <;> cases n₂ <;> try (simp [min, Option.min, Level.sub1] ; apply zero_le_all)
+        case _ n₁ n₂ =>
+          simp [Level.sub1] at hstep
+          simp
+          have h : (min (n₁ + 1) (n₂ + 1) = n₁ + 1) ∨ (min (n₁ + 1) (n₂ + 1) = n₂ + 1) := by omega
+          cases h
+          case _ h =>
+            simp [Level.sub1, h]
+            assumption
+          case _ h =>
+            simp [Level.sub1, h]
+            have h : some n₂ ≤ some n₁ := by apply le_lift ; omega
+            apply le_trans
+            repeat assumption
+  case _ =>
+    rename_i ty₁ ty₂ ty
+    cases hlub : (ty₁ ⊔ ty₂) <;> simp [hlub] at h₁
+  case _ =>
+    rename_i ty₁ ty₂
+    cases hlub : (ty₁ ⊔ ty₂) <;> simp [hlub] at h₁
+  case _ =>
+    rename_i ty₁ ty₂
+    cases hlub : (ty₁ ⊔ ty₂) <;> simp [hlub] at h₁
+  case _ =>
+    rename_i ty₁ ty₂ ety₂ l₂
+    cases hlub : (ty₁ ⊔ ty₂) <;> simp [hlub] at h₁
+  case _ =>
+    rename_i ty₁ ty₂ ty
+    cases hlub : (ty₁ ⊔ ty₂) <;> try simp [hlub] at h₁
+    subst h₁
+    cases h₂
+    rename_i set h₂
+    apply WellFormed.set
+    intros v hin
+    apply levels_lub
+    apply hlub
+    apply h₂
+    apply hin
+  case _ =>
+    rename_i ty₁ ty₂ rty
+    cases hlub : (ty₁ ⊔ ty₂) <;> simp [hlub] at h₁
+  case _ =>
+    rename_i ty₁ ty₂ rty
+    cases hlub : (ty₁ ⊔ ty₂) <;> simp [hlub] at h₁
+  case _ =>
+    not_record
+  case _ =>
+    not_record
+  case _ =>
+    not_record
+  case _ =>
+    not_record
+  case _ =>
+    not_record
+  case _ =>
+    rename_i rty₁ rty₂ rty
+
+    cases h₂
+    rename_i value_record h₃ h₄ h₅
+    cases rty₁
+    rename_i rty₁
+    cases rty₂
+    rename_i rty₂
+    cases rty
+    rename_i rty
+    have hlub : IsLubOfRecordTypes rty rty₁ rty₂ := by
+      apply lubRecordType_is_lub_of_record_types
+      simp [lub?, Option.bind] at h₁
+      cases hlubRecord : lubRecordType rty₁ rty₂ <;> simp [hlubRecord] at h₁
+      subst h₁
+      rfl
+    apply WellFormed.record
+    case _ =>
+      intros k h_contains
+      apply lubRecord_contains_left
+      apply hlub
+      apply h₃
+      apply h_contains
+    case _ =>
+      intros k v qty h_value_find h_ty_find
+      have h := lubRecord_find_implies_find hlub h_ty_find
+      have ⟨qty₁, qty₂, h_find₁, _, h_lub₁⟩ := h
+      clear h
+      have hwf : entities ⊢ v : (Qualified.getType qty₁) := by
+        apply h₅
+        repeat assumption
+      apply levels_lub
+      apply qualitype_lub_lifts
+      apply h_lub₁
+      apply hwf
+    case _ =>
+      intros k qty h_find h_isreq
+      have h := lubRecord_find_implies_find_left hlub h_find
+      have ⟨qty₁, h_find₁, h_req₁⟩ := h
+      apply h₄ k qty₁
+      apply h_find₁
+      simp [h_req₁, h_isreq]
+  case _ =>
+    not_record
+  case _ =>
+    rename_i xty₁ xty₂ xty
+    have ⟨h₂, h₃⟩ := h₁
+    subst h₂
+    subst h₃
+    assumption
+termination_by (sizeOf v)
+decreasing_by
+  all_goals simp_wf
+  all_goals (try omega)
+  case _ =>
+    rename Set Value => members
+    rename _ = (Value.set members) => heq
+    rw [heq]
+    have step₁ : sizeOf v < sizeOf (members) := by
+      apply Set.in_set_means_smaller
+      assumption
+    have step₂ : sizeOf members < sizeOf (Value.set members) := by
+      simp
+      omega
+    omega
+  case _ =>
+    rename _ = Value.record _ => heq
+    rename Map Attr Value => members
+    rw [heq]
+    have step₁ : sizeOf v < sizeOf members := by
+      apply Map.find_means_smaller
+      assumption
+    simp
+    omega
+
+theorem evaluates_to_value {v v' : Value} {e : Expr} {entities : Entities} {req : Request}
+  (h₁ : EvaluatesTo e req entities v)
+  (h₂ : evaluate e req entities = Except.ok v') :
+  v = v' := by
+  cases h₁ <;> rename_i h₁ <;> try simp [h₁] at h₂
+  cases h₁ <;> rename_i h₁ <;> try simp [h₁] at h₂
+  cases h₁ <;> rename_i h₁ <;> try simp [h₁] at h₂
+  assumption
+
+theorem eq_is_bool {lhs rhs : Expr} {c₁ c₂ : Capabilities} {ty : CedarType}  {env : Environment} {l₁ : Level}
+  (h₁ : typeOf (.binaryApp .eq lhs rhs) c₁ env (l₁ == .infinite) = Except.ok (ty, c₂)) :
+  ∃ bty, ty = .bool bty
+  := by
+  have hinv := type_of_eq_inversion h₁
+  have ⟨hinv₁, hinv₂⟩ := hinv
+  clear hinv
+  subst hinv₁
+  split at hinv₂
+  case _ =>
+    split at hinv₂
+    <;> subst hinv₂
+    <;> try (solve | exists .tt)
+    exists .ff
+  case _ =>
+    replace ⟨ty₁, _, ty₂, _, _, _, hinv₄ ⟩ := hinv₂
+    split at hinv₄
+    case _ =>
+      exists BoolType.anyBool
+    case _ =>
+      exists BoolType.ff
+      simp [hinv₄]
+
+theorem int_cmp_is_bool {o : BinaryOp} {lhs rhs : Expr} {c₁ c₂ : Capabilities} {ty : CedarType} {env : Environment} {l₁ : Level}
+  (h₁ : o = .less ∨ o = .lessEq)
+  (h₂ : typeOf (.binaryApp o rhs lhs) c₁ env (l₁ == .infinite) = Except.ok (ty, c₂)) :
+  ∃ bty, ty = .bool bty := by
+  have hinv := type_of_int_cmp_inversion h₁ h₂
+  replace ⟨_, hinv, _⟩ := hinv
+  subst hinv
+  exists .anyBool
+
+theorem int_arith_is_int {o : BinaryOp} {lhs rhs : Expr} {c₁ c₂ : Capabilities} {ty : CedarType} {env : Environment} {l₁ : Level}
+  (h₁ : o = .add ∨ o = .sub ∨ o = .mul)
+  (h₂ : typeOf (.binaryApp o rhs lhs) c₁ env (l₁ == .infinite) = Except.ok (ty, c₂)) :
+  ty = .int  := by
+  have hinv := type_of_int_arith_inversion h₁ h₂
+  simp [hinv]
+
+theorem evaluates_to_well_formed_binary {o : BinaryOp} {lhs rhs : Expr} {v : Value} {ty: CedarType} {request : Request} {entities: Entities} {env : Environment} {c₁ c₂ : Capabilities} {l₁ : Level}
+  (h₂ : RequestAndEntitiesMatchEnvironmentLeveled env request entities l₁)
+  (h₃ : typeOf (.binaryApp o lhs rhs) c₁ env (l₁ == .infinite) = Except.ok (ty, c₂))
+  (h₅ : evaluate (.binaryApp o lhs rhs) request entities = Except.ok v)
+  (h_caps : CapabilitiesInvariant c₁ request entities)
+  :
+  entities ⊢ v : ty := by
+  have hsound := (@type_of_is_sound (.binaryApp o lhs rhs))
+    (by assumption)
+    (by
+      apply request_and_entity_match_level_implies_regular
+      assumption
+    )
+    (by assumption)
+  have ⟨hsound₁, v', hsound₂, hsound₃⟩ := hsound
+  have heq : v' = v := by
+    apply evaluates_to_value
+    repeat assumption
+  subst heq
+  cases o
+  case eq =>
+    have heq := eq_is_bool h₃
+    replace ⟨bty, heq⟩ := heq
+    subst heq
+    cases hsound₃
+    apply WellFormed.bool
+    assumption
+  case mem =>
+    have hinv := type_of_mem_inversion h₃
+    have ⟨_, ety₂, l', l'', hinv₁, _, c₂', hinv₃⟩ := hinv
+    cases hinv₃
+      <;> rename_i hinv₃
+      <;> have ⟨_, hinv₄⟩ := hinv₃
+      <;> simp [typeOfInₑ, typeOfInₛ] at hinv₄
+      <;> split at hinv₄
+      <;> simp [ok, err] at hinv₄
+      <;> subst hinv₄
+      <;> cases hsound₃
+      <;> apply WellFormed.bool
+      <;> assumption
+  case less =>
+    have hbty := int_cmp_is_bool (by simp) h₃
+    replace ⟨bty, hbty⟩ := hbty
+    subst hbty
+    cases hsound₃
+    apply WellFormed.bool
+    assumption
+  case lessEq =>
+    have hbty := int_cmp_is_bool (by simp) h₃
+    replace ⟨bty, hbty⟩ := hbty
+    subst hbty
+    cases hsound₃
+    apply WellFormed.bool
+    assumption
+  case add =>
+    have hint := int_arith_is_int (by simp) h₃
+    subst hint
+    cases hsound₃
+    apply WellFormed.int
+  case sub =>
+    have hint := int_arith_is_int (by simp) h₃
+    subst hint
+    cases hsound₃
+    apply WellFormed.int
+  case mul =>
+    have hint := int_arith_is_int (by simp) h₃
+    subst hint
+    cases hsound₃
+    apply WellFormed.int
+  case contains =>
+    have hinv := type_of_contains_inversion h₃
+    have heq : ty = CedarType.bool BoolType.anyBool := by simp [hinv]
+    subst heq
+    cases hsound₃
+    apply WellFormed.bool
+    assumption
+  case containsAll =>
+    have hinv := type_of_containsA_inversion (by simp) h₃
+    have heq : ty = CedarType.bool BoolType.anyBool := by simp [hinv]
+    subst heq
+    cases hsound₃
+    apply WellFormed.bool
+    assumption
+  case containsAny =>
+    have hinv := type_of_containsA_inversion (by simp) h₃
+    have heq : ty = CedarType.bool BoolType.anyBool := by simp [hinv]
+    subst heq
+    cases hsound₃
+    apply WellFormed.bool
+    assumption
+
+theorem evaluates_to_well_formed_unary {o : UnaryOp} {x : Expr} {v : Value} {ty: CedarType} {request : Request} {entities: Entities} {env : Environment} {c₁ c₂ : Capabilities} {l₁ : Level}
+  (h₂ : RequestAndEntitiesMatchEnvironmentLeveled env request entities l₁)
+  (h₃ : typeOf (.unaryApp o x) c₁ env (l₁ == .infinite) = Except.ok (ty, c₂))
+  (h₅ : evaluate (.unaryApp o x) request entities = Except.ok v)
+  (h_caps : CapabilitiesInvariant c₁ request entities)
+  :
+  entities ⊢ v : ty := by
+  have hreq : RequestAndEntitiesMatchEnvironment env request entities := by
+    apply request_and_entity_match_level_implies_regular
+    assumption
+  have hsound := (@type_of_is_sound (.unaryApp o x)) (by assumption) (by assumption) (by assumption)
+  have ⟨hsound₁, v', hsound₂, hsound₃⟩ := hsound
+  have heq : v' = v := by
+    apply evaluates_to_value
+    repeat assumption
+  subst heq
+  clear hsound
+  cases o
+  case not =>
+    have hinv := type_of_not_inversion h₃
+    have ⟨_, bty, _, hinv₂, _⟩ := hinv
+    clear hinv
+    subst hinv₂
+    cases hsound₃
+    apply WellFormed.bool
+    assumption
+  case neg =>
+    have hinv := type_of_neg_inversion h₃
+    have ⟨_, hinv₂, _, _⟩ := hinv
+    clear hinv
+    subst hinv₂
+    cases hsound₃
+    apply WellFormed.int
+  case like =>
+    have hinv := type_of_like_inversion h₃
+    have ⟨_, hinv₂, _⟩ := hinv
+    subst hinv₂
+    cases hsound₃
+    apply WellFormed.bool
+    assumption
+  case is =>
+    have hinv := type_of_is_inversion h₃
+    have ⟨_, ety', _, _, hinv₂, _⟩ := hinv
+    clear hinv
+    rename_i _
+    split at hinv₂ <;> (
+      subst hinv₂
+      cases hsound₃
+      apply WellFormed.bool
+      assumption
+    )
+
+theorem evaluates_to_well_formed_var {v : Var} {val : Value}  {request : Request} {entities: Entities} {env : Environment} {c₁ c₂ : Capabilities} {l₁ : Level}
+  (h₂ : RequestAndEntitiesMatchEnvironmentLeveled env request entities l₁)
+  (h₃ : typeOf (.var v) c₁ env (l₁ == .infinite) = Except.ok (ty, c₂))
+  (h₅ : evaluate (.var v) request entities = Except.ok val)
+  :
+  entities ⊢ val : ty
+  := by
+  unfold RequestAndEntitiesMatchEnvironmentLeveled at h₂
+  have ⟨_, _, _, _, _, _, _⟩ := h₂
+  clear h₂
+  cases v
+    <;> simp [evaluate] at h₅
+    <;> subst h₅
+    <;> simp [typeOf, typeOfVar, ok] at h₃
+    <;> replace ⟨h₃, _⟩ := h₃
+    <;> subst h₃
+    <;> assumption
+
+theorem evaluates_to_well_formed_lit {l : Prim}  {ty: CedarType} {request : Request} {entities: Entities} {env : Environment} {c₁ c₂ : Capabilities} {l₁ : Level}
+  (h₁ : l₁ < .infinite)
+  (h₂ : RequestAndEntitiesMatchEnvironmentLeveled env request entities l₁)
+  (h₃ : typeOf (.lit l) c₁ env (l₁ == .infinite) = Except.ok (ty, c₂))
+  (h₅ : evaluate (.lit l) request entities = Except.ok v)
+  :
+  entities ⊢ v : ty := by
+  cases l <;> try (
+    rename_i value
+    cases value <;> (
+      simp [evaluate] at h₅
+      subst h₅
+      simp [typeOf, typeOfLit, ok] at h₃
+      replace ⟨h₃, _⟩ := h₃
+      subst h₃
+    )
+  )
+  case int =>
+    apply WellFormed.int
+  case bool.true =>
+    apply WellFormed.bool
+    simp [InstanceOfBoolType]
+  case bool.false =>
+    apply WellFormed.bool
+    simp [InstanceOfBoolType]
+  case string =>
+    apply WellFormed.string
+  case entityUID =>
+    rename_i euid
+    cases heq : decide (l₁ == .infinite)
+    case _ =>
+      simp at heq
+      simp [typeOf, typeOfLit] at h₃
+      split at h₃
+      case _ =>
+        simp [ok] at h₃
+        replace ⟨h₃, _⟩ := h₃
+        subst h₃
+        simp [evaluate] at h₅
+        subst h₅
+        apply WellFormed.entity₀
+        simp [InstanceOfEntityType]
+      case _ =>
+        exfalso
+        simp [err] at h₃
+    case _ =>
+      simp at heq
+      subst heq
+      cases h₁
+
+theorem set_eval_step {members : List Expr} {values : List Value}  {v : Value} {request : Request} {entities : Entities}
+ (h₁ : (members.mapM (λ x => evaluate x request entities)) = .ok values)
+ (h₂ : v ∈ values) :
+  ∃ e, e ∈ members ∧ evaluate e request entities = .ok v
+  := by
+  cases values
+  case nil =>
+    cases h₂
+  case cons head tail =>
+    cases members
+    case nil =>
+      simp [pure, Except.pure] at h₁
+    case cons members_head members_tail =>
+      cases h₂ -- Case analysis on `v ∈ (head :: tail)`
+      case _ => -- Case 1: `v = head`
+        rw [List.mapM_cons] at h₁
+        cases h_eval_head : evaluate members_head request entities <;> simp [h_eval_head] at h₁
+        rename_i head_value
+        cases h_eval_tail : List.mapM (λ x => evaluate x request entities) members_tail <;> simp [h_eval_tail] at h₁
+        rename_i values_tail
+        simp [pure, Except.pure] at h₁
+        exists members_head
+        simp [h₁, h_eval_head]
+      case _ => -- Case 2: `v ∈ tail ∧ v ≠ head`. This is the inductive case
+        rename_i hin
+        rw [List.mapM_cons] at h₁
+        cases h_eval_head : evaluate members_head request entities <;> simp [h_eval_head] at h₁
+        rename_i head_value
+        cases h_eval_tail : List.mapM (λ x => evaluate x request entities) members_tail <;> simp [h_eval_tail] at h₁
+        rename_i values_tail
+        simp [pure, Except.pure] at h₁
+        have ⟨_,  h₄⟩ := h₁
+        subst h₄
+        have ih := @set_eval_step members_tail values_tail v request entities h_eval_tail hin
+        replace⟨e, ih⟩ := ih
+        exists e
+        constructor <;> simp [ih]
+
+macro "extn_comparator_correct" f:(ident) inv:(ident) hsound₃:(ident) hsound₂:(ident) h₃:(ident) h₅:(ident) : tactic =>
+  `(tactic | (
+    have h₃ := $h₃
+    have hsound₃ := $hsound₃
+    have hsound₂ := $hsound₂
+    have h₅ := $h₅
+    have hinv := $inv (by simp [IsDecimalComparator, IsIpAddrRecognizer]) h₃
+    replace ⟨hinv, _⟩ := hinv
+    subst hinv
+    cases hsound₃
+    cases hsound₂ <;> rename_i hsound₂ <;> simp [h₅] at hsound₂
+    subst hsound₂
+    apply $f
+    assumption
+  ))
+
+macro "decimal_comparator_correct" hsound₃:(ident) hsound₂:(ident) h₃:(ident) h₅:(ident) : tactic =>
+  `(tactic | (
+    extn_comparator_correct WellFormed.bool type_of_call_decimal_comparator_inversion $hsound₃ $hsound₂ $h₃ $h₅
+  ))
+
+macro "ip_recognizer_correct" hsound₃:(ident) hsound₂:(ident) h₃:(ident) h₅:(ident) : tactic =>
+  `(tactic | (
+    extn_comparator_correct WellFormed.bool type_of_call_ipAddr_recognizer_inversion $hsound₃ $hsound₂ $h₃ $h₅
+  ))
+
+theorem evaluates_to_well_formed_call {xfn : ExtFun} {xs : List Expr} {v : Value} {ty : CedarType} {request : Request} {entities : Entities} {env : Environment} {c₁ c₂ : Capabilities} {l : Level}
+  (h₂ : RequestAndEntitiesMatchEnvironment env request entities)
+  (h₃ : typeOf (.call xfn xs) c₁ env (l == Level.infinite) = Except.ok (ty, c₂))
+  (h₅ : evaluate (.call xfn xs) request entities = Except.ok v)
+  (h_caps : CapabilitiesInvariant c₁ request entities) :
+  entities ⊢ v : ty
+  := by
+  have hsound := (@type_of_is_sound (.call xfn xs))
+    (by assumption)
+    (by assumption)
+    (by assumption)
+  have ⟨hsound₁, v, hsound₂, hsound₃⟩ := hsound
+  clear hsound
+  cases xfn
+  case decimal =>
+    have hinv := type_of_call_decimal_inversion h₃
+    replace ⟨hinv, _⟩ := hinv
+    subst hinv
+    cases hsound₃
+    cases hsound₂ <;> rename_i hsound₂ <;> simp [h₅] at hsound₂
+    subst hsound₂
+    apply WellFormed.ext
+    assumption
+  case lessThan =>
+    decimal_comparator_correct hsound₃ hsound₂ h₃ h₅
+  case lessThanOrEqual =>
+    decimal_comparator_correct hsound₃ hsound₂ h₃ h₅
+  case greaterThan =>
+    decimal_comparator_correct hsound₃ hsound₂ h₃ h₅
+  case greaterThanOrEqual =>
+    decimal_comparator_correct hsound₃ hsound₂ h₃ h₅
+  case ip =>
+    have hinv := type_of_call_ip_inversion h₃
+    replace ⟨hinv, _⟩ := hinv
+    subst hinv
+    cases hsound₃
+    cases hsound₂ <;> rename_i hsound₂ <;> simp [h₅] at hsound₂
+    subst hsound₂
+    apply WellFormed.ext
+    assumption
+  case isIpv4 =>
+    ip_recognizer_correct hsound₃ hsound₂ h₃ h₅
+  case isIpv6 =>
+    ip_recognizer_correct hsound₃ hsound₂ h₃ h₅
+  case isLoopback =>
+    ip_recognizer_correct hsound₃ hsound₂ h₃ h₅
+  case isMulticast =>
+    ip_recognizer_correct hsound₃ hsound₂ h₃ h₅
+  case isInRange =>
+    have hinv := type_of_call_isInRange_inversion h₃
+    replace ⟨hinv, _⟩ := hinv
+    subst hinv
+    cases hsound₃
+    cases hsound₂ <;> rename_i hsound₂ <;> simp [h₅] at hsound₂
+    subst hsound₂
+    apply WellFormed.bool
+    assumption
+
+theorem evaluates_to_well_formed_ite {cond cons alt : Expr} {v : Value} {request : Request} {entities : Entities} {c₁ c₂ : Capabilities} {l₁ : Level}
+  (h₁ : l₁ < .infinite)
+  (h₂ : RequestAndEntitiesMatchEnvironmentLeveled env request entities l₁)
+  (h₃ : typeOf (.ite cond cons alt) c₁ env (l₁ == .infinite) = Except.ok (ty, c₂))
+  (h₅ : evaluate (.ite cond cons alt) request entities = Except.ok v)
+  (h_caps : CapabilitiesInvariant c₁ request entities)
+  (ih₁ : EvaluatesToWellFormed cons)
+  (ih₂ : EvaluatesToWellFormed alt) :
+  entities ⊢ v : ty := by
+  have hsound : GuardedCapabilitiesInvariant (.ite cond cons alt) c₂ request entities ∧ ∃ v, EvaluatesTo (.ite cond cons alt) request entities v ∧ InstanceOfType v ty := by
+    type_soundness
+  have ⟨hsound₁, v', hsound₂, hsound₃⟩ := hsound
+  clear hsound
+  dril_to_value hsound₂ h₅
+  have hinv := type_of_ite_inversion h₃
+  replace ⟨bty, c₁', ty₂, c₂', ty₃, c₃, hinv₁, hinv⟩ := hinv
+  have hsound_cond : GuardedCapabilitiesInvariant cond c₁' request entities ∧ ∃ v, EvaluatesTo cond request entities v ∧ InstanceOfType v (.bool bty)  := by
+    type_soundness
+  have ⟨hsound_cond₁, v_cond, hsound_cond₂, hsound_cond₃⟩ := hsound_cond
+  clear hsound_cond
+  have heval_cond : ∃ v, evaluate cond request entities = Except.ok v := by
+    cases hcond : evaluate cond request entities
+    case error =>
+      simp [evaluate, hcond, Result.as] at h₅
+    case ok v =>
+      exists v
+  replace ⟨v_cond, heval_cond⟩ := heval_cond
+  dril_to_value hsound_cond₂ heval_cond
+  cases hsound_cond₃
+  rename_i bool_val hsound_cond₃
+  cases bty
+  case tt =>
+    simp at hinv
+    have ⟨hinv₂, hinv₃, _⟩ := hinv
+    clear hinv
+    subst hinv₃
+    cases bool_val <;> simp [InstanceOfBoolType] at hsound_cond₃
+    apply ih₁
+    repeat assumption
+    simp [evaluate, heval_cond, Result.as, Coe.coe, Value.asBool] at h₅
+    assumption
+    apply capability_union_invariant
+    assumption
+    apply hsound_cond₁
+    assumption
+  case ff =>
+    simp at hinv
+    have ⟨hinv₂, hinv₃, hinv₄⟩ := hinv
+    clear hinv
+    subst hinv₃
+    subst hinv₄
+    cases bool_val <;> simp [InstanceOfBoolType] at hsound_cond₃
+    apply ih₂
+    repeat assumption
+    simp [evaluate, heval_cond, Result.as, Coe.coe, Value.asBool] at h₅
+    repeat assumption
+  case anyBool =>
+    simp at hinv
+    have ⟨hinv₁, hinv₂, hinv₃, hinv₄⟩ := hinv
+    clear hinv
+    subst hinv₄
+    cases bool_val
+    case true =>
+      have hsound_cons : GuardedCapabilitiesInvariant cons c₂' request entities ∧ ∃ v, EvaluatesTo cons request entities v ∧ InstanceOfType v ty₂ := by
+        apply type_of_is_sound
+        apply capability_union_invariant
+        assumption
+        apply hsound_cond₁
+        assumption
+        apply request_and_entity_match_level_implies_regular
+        assumption
+        assumption
+      have ⟨_, v_cons, hsound_cons₂, _⟩ := hsound_cons
+      clear hsound_cons
+      have heval_cons : ∃ v, evaluate cons request entities = .ok v := by
+        cases h : evaluate cons request entities
+        case ok v =>
+          exists v
+        case error =>
+          simp [evaluate, heval_cond, h, Result.as, Coe.coe, Value.asBool] at h₅
+      replace ⟨v_cons', heval_cons⟩ := heval_cons
+      dril_to_value hsound_cons₂ heval_cons
+      simp [heval_cons, heval_cond, evaluate, Result.as, Coe.coe, Value.asBool] at h₅
+      subst h₅
+      have step : (entities ⊢ v_cons : ty₂) := by
+        apply ih₁
+        assumption
+        assumption
+        assumption
+        assumption
+        apply capability_union_invariant
+        assumption
+        apply hsound_cond₁
+        assumption
+      apply levels_lub
+      repeat assumption
+    case false =>
+
+      have hsound_alt : GuardedCapabilitiesInvariant alt c₃ request entities ∧ ∃ v, EvaluatesTo alt request entities v ∧ InstanceOfType v ty₃ := by
+        type_soundness
+      have ⟨hsound_alt₁, v_alt, hsound_alt₂, hsound_alt₃⟩ := hsound_alt
+      clear hsound_alt
+      have heval_alt : ∃ v, evaluate alt request entities = .ok v := by
+        cases h : evaluate alt request entities
+        case ok v =>
+          exists v
+        case error =>
+          simp [evaluate, h, heval_cond, Result.as, Coe.coe, Value.asBool] at h₅
+      replace ⟨v_alt', heval_alt⟩ := heval_alt
+      dril_to_value hsound_alt₂ heval_alt
+      simp [evaluate, heval_alt, heval_cond, Result.as, Coe.coe, Value.asBool] at h₅
+      subst h₅
+      have step : entities ⊢ v_alt : ty₃ := by
+        apply ih₂
+        repeat assumption
+      apply levels_lub
+      rw [lub_comm] at hinv₃
+      repeat assumption
+
+macro "bool_constant" hinv:(ident) hsound₃:(ident) : tactic =>
+  `(tactic | (
+    solve | (
+      have hinv := $hinv
+      have hsound₃ := $hsound₃
+      simp [lubBool] at hinv
+      have ⟨hinv₁, hinv₂, hinv₃⟩ := hinv
+      subst hinv₂
+      cases hsound₃
+      rename_i bool_val hsound₃
+      cases bool_val <;> simp [InstanceOfBoolType] at hsound₃
+      apply WellFormed.bool
+      assumption
+    )
+  ))
+
+theorem evaluates_to_well_formed_and {lhs rhs : Expr} {v : Value} {request : Request} {entities : Entities} {c₁ c₂ : Capabilities} {l₁ : Level}
+  (h₂ : RequestAndEntitiesMatchEnvironmentLeveled env request entities l₁)
+  (h₃ : typeOf (.and lhs rhs) c₁ env (l₁ == .infinite) = Except.ok (ty, c₂))
+  (h₅ : evaluate (.and lhs rhs) request entities = Except.ok v)
+  (h_caps : CapabilitiesInvariant c₁ request entities) :
+  entities ⊢ v : ty := by
+  have hsound : GuardedCapabilitiesInvariant (.and lhs rhs) c₂ request entities ∧ ∃ v, EvaluatesTo (.and lhs rhs) request entities v ∧ InstanceOfType v ty
+  := by type_soundness
+  have ⟨_, v', hsound₂, hsound₃⟩ := hsound
+  clear hsound
+  dril_to_value hsound₂ h₅
+  have hinv := type_of_and_inversion h₃
+  replace ⟨bty, c₁', hinv⟩ := hinv
+  cases bty
+  case tt =>
+    simp at hinv
+    replace ⟨_, bty₂, c₂', hinv⟩ := hinv
+    cases bty₂ <;> bool_constant hinv hsound₃
+  case ff =>
+    simp at hinv
+    bool_constant hinv hsound₃
+  case anyBool =>
+    simp at hinv
+    replace ⟨_, bty₂, c₂', hinv⟩ := hinv
+    cases bty₂ <;> simp at hinv <;> bool_constant hinv hsound₃
+
+theorem evaluates_to_well_formed_or {lhs rhs : Expr} {v : Value} {request : Request} {entities : Entities} {c₁ c₂ : Capabilities} {l₁ : Level}
+  (h₂ : RequestAndEntitiesMatchEnvironmentLeveled env request entities l₁)
+  (h₃ : typeOf (.or lhs rhs) c₁ env (l₁ == .infinite) = Except.ok (ty, c₂))
+  (h₅ : evaluate (.or lhs rhs) request entities = Except.ok v)
+  (h_caps : CapabilitiesInvariant c₁ request entities) :
+  entities ⊢ v : ty := by
+  have hsound : GuardedCapabilitiesInvariant (.or lhs rhs) c₂ request entities ∧ ∃ v, EvaluatesTo (.or lhs rhs) request entities v ∧ InstanceOfType v ty := by
+    type_soundness
+  have ⟨_, v', hsound₂, hsound₃⟩ := hsound
+  clear hsound
+  dril_to_value hsound₂ h₅
+  have hinv := type_of_or_inversion h₃
+  replace ⟨bty₁, c₁', hinv⟩ := hinv
+  cases bty₁
+  case tt =>
+    bool_constant hinv hsound₃
+  case ff =>
+    simp at hinv
+    replace ⟨_, bty₂, hinv⟩ := hinv
+    cases bty₂
+    case ff =>
+      have ⟨_, hinv₂⟩ := hinv
+      clear hinv
+      subst hinv₂
+      cases hsound₃
+      rename_i bool hsound₃
+      cases bool <;> simp [InstanceOfBoolType] at hsound₃
+      apply WellFormed.bool
+      assumption
+    case tt =>
+      have ⟨_, hinv₂⟩ := hinv
+      clear hinv
+      subst hinv₂
+      cases hsound₃
+      rename_i bool hsound₃
+      cases bool <;> simp [InstanceOfBoolType] at hsound₃
+      apply WellFormed.bool
+      assumption
+    case anyBool =>
+      have ⟨_, hinv₂⟩ := hinv
+      clear hinv
+      subst hinv₂
+      cases hsound₃
+      rename_i bool hsound₃
+      cases bool <;> simp [InstanceOfBoolType] at hsound₃
+      <;> apply WellFormed.bool
+      <;> assumption
+  case anyBool =>
+    simp at hinv
+    replace ⟨_, bty₂, c₂', hinv⟩ := hinv
+    cases bty₂ <;> bool_constant hinv hsound₃
+
+theorem evaluates_to_well_formed_getAttr_entity {e : Expr} {attr : Attr} {v : Value} {request : Request} {entities : Entities} {env : Environment} {c₁ c₁' : Capabilities} {l₁ l₂ : Level} {ety : EntityType}
+  (h₁ : l₁ < .infinite)
+  (h₂ : RequestAndEntitiesMatchEnvironmentLeveled env request entities l₁)
+  (h₄ : evaluate (.getAttr e attr) request entities = .ok v)
+  (h₅ : CapabilitiesInvariant c₁ request entities)
+  (h₆ : typeOf e c₁ env (l₁ == Level.infinite) = Except.ok (CedarType.entity ety l₂, c₁'))
+  (h₇ : l₂ > Level.finite 0)
+  (ih : EvaluatesToWellFormed e) :
+  (entities ⊢ v : ty) := by
+  have hsound : GuardedCapabilitiesInvariant e c₁' request entities ∧ ∃ v, EvaluatesTo e request entities v ∧ InstanceOfType v (.entity ety l₂) := by
+    type_soundness
+  have ⟨_, v_entity, hsound₂, hsound₃⟩ := hsound
+  have heval : ∃ v_entity', evaluate e request entities = .ok v_entity' := by
+    cases h : evaluate e request entities
+    case ok v =>
+      exists v
+    case error =>
+      simp [evaluate, Result.as, h] at h₄
+  replace ⟨v_entity', heval⟩ := heval
+  dril_to_value hsound₂ heval
+  cases hsound₃
+  rename_i euid hsound₃
+  have step : entities ⊢ (.prim (.entityUID euid)) : .entity ety l₂ := by
+    apply ih
+    repeat assumption
+  cases step -- Two ways to have a well formed entity value
+  case _ => -- The level can be zero, which is impossible as we're derefing ijt
+    cases h₇
+    omega
+  case _ => -- The level can be nonzero
+    rename_i attrs ih₁ ih₂ ih₃ ih₄
+    apply ih₁
+    simp [getAttr, attrsOf, ih₁, evaluate, heval, ih₂] at h₄
+    apply Map.findOrErr_ok_implies_in_kvs
+    apply h₄
+
+theorem evaluates_to_well_formed_getAttr_record {e : Expr} {attr : Attr} {v : Value} {request : Request} {entities : Entities} {env : Environment} {c₁ c₂ c₁' : Capabilities} {l₁ : Level} {rty : RecordType}
+  (h₁ : l₁ < .infinite)
+  (h₂ : RequestAndEntitiesMatchEnvironmentLeveled env request entities l₁)
+  (h₃ : typeOf (.getAttr e attr) c₁ env (l₁ == .infinite) = .ok (ty, c₂))
+  (h₄ : evaluate (.getAttr e attr) request entities = .ok v)
+  (h₅ : CapabilitiesInvariant c₁ request entities)
+  (h₆ : typeOf e c₁ env (l₁ == Level.infinite) = Except.ok (CedarType.record rty, c₁'))
+  (ih : EvaluatesToWellFormed e) :
+  (entities ⊢ v : ty) := by
+  have hsound : GuardedCapabilitiesInvariant e c₁' request entities ∧ ∃ v, EvaluatesTo e request entities v ∧ InstanceOfType v (.record rty) := by
+    type_soundness
+  have ⟨_, v_record, hsound₂, hsound₃⟩ := hsound
+  clear hsound
+  have heval : ∃ v_record', evaluate e request entities = .ok v_record' := by
+    cases h: evaluate e request entities
+    case ok v =>
+      exists v
+    case error _ =>
+      simp [h, evaluate, Result.as] at h₄
+  replace ⟨v_record', heval⟩ := heval
+  dril_to_value hsound₂ heval
+  cases hsound₃
+  rename_i record hsound₃₁ hsound₃₂ hsound₃₃
+  have step : entities ⊢ (Value.record record) : .record rty := by
+    apply ih
+    repeat assumption
+  cases step
+  rename_i ih₁ ih₂ ih₃
+  simp [evaluate, getAttr, attrsOf, heval] at h₄
+  have hcontains : rty.contains attr = true := by
+    apply hsound₃₁
+    simp [Map.contains]
+    cases h : record.find? attr
+    case a.some =>
+      simp
+    case a.none =>
+      simp [Map.findOrErr, h] at h₄
+  have hqty : ∃ (qty : QualifiedType), rty.find? attr = .some qty := by
+    simp [Map.contains] at hcontains
+    cases h : Map.find? rty attr
+    case none =>
+      simp [h] at hcontains
+    case some qty =>
+      exists qty
+  replace ⟨qty, hqty⟩ := hqty
+  have heq : qty.getType = ty := by
+    simp [typeOf, h₆, typeOfGetAttr, getAttrInRecord, hqty] at h₃
+    cases qty
+    case _ =>
+      simp at h₃
+      cases hin : decide ((e,attr) ∈ c₁) <;> simp at hin
+      case _ =>
+        rw [if_neg] at h₃
+        simp [err] at h₃
+        assumption
+      case _ =>
+        rw [if_pos] at h₃
+        rename_i ty'
+        simp [ok] at h₃
+        replace ⟨h₃, _⟩ := h₃
+        subst h₃
+        simp [Qualified.getType]
+        assumption
+    case _ =>
+      rename_i ty'
+      simp [ok] at h₃
+      replace ⟨h₃, _⟩ := h₃
+      subst h₃
+      simp [Qualified.getType]
+  have step := ih₃ attr v qty
+    (by
+      cases h : record.find? attr <;> simp [h, Map.findOrErr] at h₄
+      subst h₄
+      rfl
+    )
+    hqty
+  rw [heq] at step
+  assumption
+
+theorem evaluates_to_well_formed_getAttr {e : Expr} {attr : Attr} {v : Value} {request : Request} {entities : Entities} {env : Environment} {c₁ c₂ : Capabilities} {l₁ : Level}
+  (h₁ : l₁ < .infinite)
+  (h₂ : RequestAndEntitiesMatchEnvironmentLeveled env request entities l₁)
+  (h₃ : typeOf (.getAttr e attr) c₁ env (l₁ == .infinite) = .ok (ty, c₂))
+  (h₄ : evaluate (.getAttr e attr) request entities = .ok v)
+  (h₅ : CapabilitiesInvariant c₁ request entities)
+  (ih : EvaluatesToWellFormed e) :
+  entities ⊢ v : ty := by
+  have hsound : GuardedCapabilitiesInvariant (.getAttr e attr) c₂ request entities ∧ ∃ v, EvaluatesTo (.getAttr e attr) request entities v ∧  InstanceOfType v ty := by
+    type_soundness
+  have ⟨hsound₁, v', hsound₂, _⟩ := hsound
+  clear hsound
+  dril_to_value hsound₂ h₄
+  have hinv := type_of_getAttr_inversion_levels h₃
+  replace ⟨hinv₁, c₁', hinv⟩ := hinv
+  subst hinv₁
+  cases hinv <;> rename_i hinv
+  case _ =>
+    replace ⟨ety, l₂, hinv₁, hinv₂⟩ := hinv
+    clear hinv
+    apply evaluates_to_well_formed_getAttr_entity
+    repeat assumption
+  case _ =>
+    replace ⟨rty, hinv⟩ := hinv
+    apply evaluates_to_well_formed_getAttr_record
+    repeat assumption
+
+theorem levels_correct_hasAttr {e : Expr} {attr : Attr} {v : Value} {request : Request} {entities : Entities} {env : Environment} {c₁ c₂ : Capabilities} {l₁ : Level}
+  (h₂ : RequestAndEntitiesMatchEnvironmentLeveled env request entities l₁)
+  (h₃ : typeOf (.hasAttr e attr) c₁ env (l₁ == .infinite) = .ok (ty, c₂))
+  (h₄ : evaluate (.hasAttr e attr) request entities = .ok v)
+  (h₅ : CapabilitiesInvariant c₁ request entities) :
+  entities ⊢ v : ty := by
+  have hsound : GuardedCapabilitiesInvariant (.hasAttr e attr) c₂ request entities ∧ ∃ v, EvaluatesTo (.hasAttr e attr) request entities v ∧ InstanceOfType v ty := by
+    type_soundness
+  have ⟨_, v', hsound₂, hsound₃⟩ := hsound
+  dril_to_value hsound₂ h₄
+  have hinv := type_of_hasAttr_inversion' h₃
+  replace ⟨bty, hinv⟩ := hinv
+  subst hinv
+  cases bty <;> try (
+    solve | (
+    cases hsound₃
+    rename_i bool hsound₃
+    cases bool <;> simp [InstanceOfBoolType] at hsound₃
+    apply WellFormed.bool
+    assumption
+    )
+  )
+  case anyBool =>
+    cases hsound₃
+    apply WellFormed.bool
+    assumption
+
+theorem levels_correct_set {members : List Expr} {v : Value} {request : Request} {entities : Entities} {env : Environment} {c₁ c₂ : Capabilities} {l₁ : Level}
+  (h₁ : l₁ < .infinite)
+  (h₂ : RequestAndEntitiesMatchEnvironmentLeveled env request entities l₁)
+  (h₃ : typeOf (.set members) c₁ env (l₁ == .infinite) = Except.ok (ty, c₂))
+  (h₄ : evaluate (.set members) request entities = .ok v)
+  (h₅ : CapabilitiesInvariant c₁ request entities)
+  (ih : ∀ e, e ∈ members → EvaluatesToWellFormed e) :
+  entities ⊢ v : ty := by
+  have hsound : GuardedCapabilitiesInvariant (.set members) c₂ request entities ∧ ∃ v, EvaluatesTo (.set members) request entities v ∧ InstanceOfType v ty := by
+    type_soundness
+  have ⟨hsound₁, v', hsound₂, hsound₃⟩ := hsound
+  clear hsound
+  dril_to_value hsound₂ h₄
+  have hinv := type_of_set_inversion h₃
+  have ⟨hinv₁, ty', hinv₂, hinv₃⟩ := hinv
+  clear hinv
+  subst hinv₂
+  subst hinv₁
+  cases hsound₃
+  rename_i set_value hinst
+  apply WellFormed.set
+  intros v hin
+  simp [evaluate, List.mapM₁, List.attach, List.attachWith] at h₄
+  rw [List.mapM_pmap_subtype (λ (e : Expr) => evaluate e request entities) members] at h₄
+  cases hmembers : List.mapM (λ e => evaluate e request entities) members <;> simp [hmembers] at h₄
+  rename_i member_list
+  have in_list : v ∈ member_list := by
+    apply Set.in_constructor_in_set
+    rw [h₄]
+    assumption
+  have hexpr := (@set_eval_step members member_list) hmembers in_list
+  have ⟨e, hexpr₁, hexpr₂⟩ := hexpr
+  clear hexpr
+  have hinv₄ := hinv₃ e hexpr₁
+  replace ⟨tyᵢ, cᵢ, hinv₄, hinv₅⟩ := hinv₄
+  have step : entities ⊢ v : tyᵢ := by
+    apply ih
+    repeat assumption
+  apply levels_lub
+  repeat assumption
+
+theorem record_eval_step (attrs : List (Attr × Expr)) (record : List (Attr × Value)) (request : Request) (entities : Entities) (attr : Attr) (v : Value)
+  (h₁ : List.mapM (λ (pair : (Attr × Expr)) => bindAttr pair.fst (evaluate pair.snd request entities)) attrs = .ok record)
+  (h₂ : (attr, v) ∈ record) :
+  ∃ e, (attr, e) ∈ attrs ∧ evaluate e request entities = .ok v := by
+  cases attrs <;> cases record
+  case _ =>
+    cases h₂
+  case _ =>
+    simp [List.mapM, List.mapM.loop, pure, Except.pure] at h₁
+  case _ =>
+    cases h₂
+  case _ attr_head attr_tail record_head record_tail =>
+    rw [List.mapM_cons] at h₁
+    cases hhead : bindAttr attr_head.fst (evaluate attr_head.snd request entities) <;> simp [hhead] at h₁
+    cases htail : List.mapM (λ pair => bindAttr pair.fst (evaluate pair.snd request entities)) attr_tail <;> simp [htail] at h₁
+    rename_i head tail
+    cases h₂
+    case _ =>
+      cases head
+      simp [pure, Except.pure] at h₁
+      have ⟨⟨heq₁, heq₂⟩, heq₃⟩ := h₁
+      subst heq₁
+      subst heq₂
+      subst heq₃
+      rename_i attr v
+      clear h₁
+      have ⟨attr', e⟩ := attr_head
+      exists e
+      simp [bindAttr] at hhead
+      cases heval : evaluate e request entities <;> simp [heval] at hhead
+      simp [hhead]
+    case _ hin =>
+      simp [pure, Except.pure] at h₁
+      simp [h₁] at htail
+      have ih := record_eval_step attr_tail record_tail request entities attr v htail hin
+      replace ⟨e, ih⟩ := ih
+      exists e
+      simp [ih]
+
+theorem forall₂_find_match {α β : Type} (l₁ : List α) (l₂ : List β) (p : α → β → Prop) (a : α)
+  (h₁ : List.Forall₂ p l₁ l₂)
+  (h₂ : a ∈ l₁) :
+  ∃ b, b ∈ l₂ ∧ p a b
+  := by
+  cases h₁
+  case nil =>
+    cases h₂
+  case cons =>
+    rename_i a_head b_head a_tail b_tail holds_on_head holds_on_tail
+    cases h₂
+    case _ =>
+      exists b_head
+      simp [holds_on_head]
+    case _ hin =>
+      have ih := forall₂_find_match a_tail b_tail p a holds_on_tail hin
+      replace ⟨b, ih₁, ih₂⟩ := ih
+      exists b
+      simp [ih₁, ih₂]
+
+theorem AttrExprHasAttrType_constraints_keys (k₁ k₂ : Attr) (e : Expr) (qty : QualifiedType) (c : Capabilities) (env : Environment) (l : Level)
+  (h₁ : AttrExprHasAttrType c env l (k₁, e) (k₂, qty)) :
+  k₁ = k₂ := by
+  simp [AttrExprHasAttrType] at h₁
+  have ⟨_, h₁⟩ := h₁
+  simp [h₁]
+
+theorem evaluate_empty_record (request : Request) (entities : Entities) :
+  evaluate (.record []) request entities = .ok (Value.record (Map.make [])) := by
+  simp [evaluate, List.mapM₂, List.attach₂]
+
+theorem evaluates_to_well_formed_record {attrs : List (Attr × Expr)} {v : Value} {request : Request} {entities : Entities} {env : Environment} {c₁ c₂ : Capabilities} {l₁ : Level}
+  (h₁ : l₁ < .infinite)
+  (h₂ : RequestAndEntitiesMatchEnvironmentLeveled env request entities l₁)
+  (h₃ : typeOf (.record attrs) c₁ env (l₁ == .infinite) = Except.ok (ty, c₂))
+  (h₅ : evaluate (.record attrs) request entities = Except.ok v)
+  (h_caps : CapabilitiesInvariant c₁ request entities)
+  (ih : ∀ (a : Attr) (e : Expr), (a,e) ∈ attrs → EvaluatesToWellFormed e ) :
+  entities ⊢ v : ty := by
+  have hsound : GuardedCapabilitiesInvariant (.record attrs) c₂ request entities ∧ ∃ v, EvaluatesTo (.record attrs) request entities v ∧ InstanceOfType v ty := by
+    type_soundness
+  have ⟨hsound₁, v', hsound₂, hsound₃⟩ := hsound
+  clear hsound
+  dril_to_value hsound₂ h₅
+  clear hsound₂
+  have hinv := type_of_record_inversion h₃
+  replace ⟨_, rty, hinv₁, hinv⟩ := hinv
+  subst hinv₁
+  cases hsound₃
+  rename_i attr_map hsound₃ hsound₄ hsound₅
+  cases attrs
+  case nil =>
+    cases hinv
+    simp [evaluate_empty_record, Map.make, List.canonicalize] at h₅
+    rw [← h₅]
+    apply WellFormed.record
+    case _ =>
+      intros k  hcontains
+      simp [Map.contains, Map.find?, List.find?] at hcontains
+    case _ =>
+      intros k v qty hfind_value hfind_type
+      simp [Map.find?, List.find?] at hfind_value
+    case _ =>
+      intros k qty hfind
+      simp [Map.find?, List.find?] at hfind
+  case cons attr attrs =>
+    sorry
+
+theorem evaluates_to_well_formed {x : Expr} {v : Value} {ty: CedarType} {request : Request} {entities: Entities} {env : Environment} {c₁ c₂ : Capabilities} {l₁ : Level}
+  (h₁ : l₁ < .infinite)
+  (h₂ : RequestAndEntitiesMatchEnvironmentLeveled env request entities l₁)
+  (h₃ : typeOf x c₁ env (l₁ == .infinite) = Except.ok (ty, c₂))
+  (h₅ : evaluate x request entities = Except.ok v)
+  (h_caps : CapabilitiesInvariant c₁ request entities)
+  :
+  entities ⊢ v : ty
+  := by
+  have hreq : RequestAndEntitiesMatchEnvironment env request entities :=  by
+    apply request_and_entity_match_level_implies_regular
+    assumption
+  cases x
+  case lit p =>
+    apply evaluates_to_well_formed_lit
+    repeat assumption
+  case var x =>
+    apply evaluates_to_well_formed_var
+    repeat assumption
+  case ite cond cons alt =>
+    apply evaluates_to_well_formed_ite
+    repeat assumption
+    case ih₁ =>
+      simp [EvaluatesToWellFormed]
+      intros
+      apply evaluates_to_well_formed
+      repeat assumption
+    case ih₂ =>
+      simp [EvaluatesToWellFormed]
+      intros
+      apply evaluates_to_well_formed
+      repeat assumption
+  case _ lhs rhs => -- and
+    apply evaluates_to_well_formed_and
+    repeat assumption
+  case _ lhs rhs => -- or
+    apply evaluates_to_well_formed_or
+    repeat assumption
+  case _ op expr => -- unary ops
+    apply evaluates_to_well_formed_unary
+    repeat assumption
+  case _ o lhs rhs => -- binary ops
+    apply evaluates_to_well_formed_binary
+    repeat assumption
+  case _ => --get attr
+    apply evaluates_to_well_formed_getAttr
+    repeat assumption
+    simp [EvaluatesToWellFormed]
+    intros
+    apply evaluates_to_well_formed
+    repeat assumption
+  case hasAttr expr attr =>
+    apply levels_correct_hasAttr
+    repeat assumption
+  case set members =>
+    apply levels_correct_set
+    repeat assumption
+    intros
+    simp [EvaluatesToWellFormed]
+    intros
+    apply evaluates_to_well_formed
+    repeat assumption
+  case record attrs =>
+    apply evaluates_to_well_formed_record
+    repeat assumption
+    intros _ e _
+    simp [EvaluatesToWellFormed]
+    intros
+    apply evaluates_to_well_formed
+    repeat assumption
+  case call xfn args =>
+    apply evaluates_to_well_formed_call
+    repeat assumption
+termination_by (sizeOf x)
+decreasing_by
+  all_goals simp_wf
+  all_goals (try omega)
+  case _ =>
+    rename_i heq _ _ _ _ _ _ _ _ _ _ _ _ _
+    rw [heq]
+    simp
+    omega
+  case _ =>
+    rename_i heq _ _ _ _ _ _ _ _ _ _ _ _ _
+    rw [heq]
+    simp
+    omega
+  case _ =>
+    rename_i heq _ _ _ _ _ _ _ _ _ _ _ _ _
+    rw [heq]
+    simp
+    omega
+  case _ =>
+    rename_i members heq e hin _ _ _ _ _ _ _ _ _ _ _ _ _
+    rw [heq]
+    have hstep : sizeOf e < sizeOf members := by
+      apply List.in_lists_means_smaller e members
+      assumption
+    simp
+    omega
+  case _ =>
+    rename_i members heq a hin _ _ _ _ _ _ _ _ _ _ _ _ _
+    rw [heq]
+    have step1 : sizeOf e < sizeOf (a,e) := by
+      simp
+      omega
+    have step2 : sizeOf (a,e) < sizeOf members := by
+      apply List.in_lists_means_smaller
+      assumption
+    simp
+    omega
+
+end Cedar.Thm
